template-coq/theories/Typing.v
@@ -810,7 +810,7 @@ Inductive typing `{checker_flags} (Σ : global_env_ext) (Γ : context) : term ->
     consistent_instance_ext Σ (ind_universes mdecl) p.(puinst) ->
     let predctx := case_predicate_context ci.(ci_ind) mdecl idecl p in
     Σ ;;; Γ ,,, predctx |- p.(preturn) : tSort ps ->
-    is_allowed_elimination Σ ps idecl.(ind_kelim) ->
+    is_allowed_elimination Σ idecl.(ind_kelim) ps ->
     Σ ;;; Γ |- c : mkApps (tInd ci.(ci_ind) p.(puinst)) (p.(pparams) ++ indices) ->
     isCoFinite mdecl.(ind_finite) = false ->
     let ptm := it_mkLambda_or_LetIn predctx p.(preturn) in
@@ -1169,7 +1169,7 @@ Lemma typing_ind_env `{cf : checker_flags} :
         forall pret : Σ ;;; Γ ,,, predctx |- p.(preturn) : tSort ps,
         P Σ (Γ ,,, predctx) p.(preturn) (tSort ps) ->
         PΓ Σ (Γ ,,, predctx) (typing_wf_local pret) ->
-        is_allowed_elimination Σ ps idecl.(ind_kelim) ->
+        is_allowed_elimination Σ idecl.(ind_kelim) ps ->
         Σ ;;; Γ |- c : mkApps (tInd ci.(ci_ind) p.(puinst)) (p.(pparams) ++ indices) ->
         P Σ Γ c (mkApps (tInd ci.(ci_ind) p.(puinst)) (p.(pparams) ++ indices)) ->
         isCoFinite mdecl.(ind_finite) = false ->
